Updated compilation for new [get_env] definition.
[get_env] now includes operational specifications of methods when
generating a module's calling environments (as opposed to just their
axiomatic specs). ADT compilation now accounts for this extended
environment by parameterizing over an arbitrary extension of operational
specifications, as we're generating the method bodies used in these
specifications as part of the translation step.

src/CertifiedExtraction/ADT2CompileUnit.v
@@ -12,6 +12,56 @@ Require Import
         CertifiedExtraction.Extraction.Internal
         CertifiedExtraction.Extraction.Extraction.
 
+Add Parametric Morphism av
+  : (@RunsTo av)
+    with signature
+    (GLabelMapFacts.Submap ==> eq ==> StringMap.Equal ==> StringMap.Equal ==> impl)
+      as Proper_RunsTo.
+Proof.
+  unfold impl; intros.
+  revert y y1 y2 H0 H1 H.
+  induction H2; intros.
+  - econstructor; rewrite <- H0, <- H1; eauto.
+  - econstructor 2; eauto.
+    eapply IHRunsTo1; eauto.
+    reflexivity.
+    eapply IHRunsTo2; eauto.
+    reflexivity.
+  - econstructor 3; eauto.
+    unfold is_true, eval_bool.
+    setoid_rewrite <- H0; apply H.
+  - econstructor 4; eauto.
+    unfold is_false, eval_bool.
+    setoid_rewrite <- H0; apply H.
+  - econstructor 5; eauto.
+    unfold is_true, eval_bool.
+    setoid_rewrite <- H0; apply H.
+    eapply IHRunsTo1; eauto.
+    reflexivity.
+    eapply IHRunsTo2; eauto.
+    reflexivity.
+  - econstructor 6; eauto.
+    unfold is_false, eval_bool.
+    setoid_rewrite <- H1; apply H.
+    rewrite <- H1, <- H2; eauto.
+  - econstructor 7;
+    rewrite <- H2; eauto.
+    rewrite <- H1; symmetry; eauto.
+  - econstructor 8; eauto.
+    rewrite <- H6; eauto.
+    rewrite <- H6; eauto.
+    rewrite <- H7.
+    subst st'; subst st'0; rewrite <- H6; eauto.
+  - econstructor 9; eauto.
+    rewrite <- H7; eauto.
+    rewrite <- H7; eauto.
+    eapply IHRunsTo; eauto.
+    reflexivity.
+    reflexivity.
+    subst st'; subst st'0; subst output; rewrite <- H8.
+    rewrite <- H7; eauto.
+Qed.
+
 Record GoodWrapper av A :=
   { gWrap : FacadeWrapper (Value av) A;
     gWrapTag : bool;
@@ -524,7 +574,9 @@ Definition BuildCompileUnit2TSpec
 
 Lemma BuildDFFun_is_syntax_ok
       av
-      (env : Env av)
+      (* The calling environment is parameterized over an extension *)
+      (* representing the operational specifications of the module. *)
+      (env : StringMap.t DFFun -> Env av)
       {WrappedRepT RepT}
       cod
       dom
@@ -536,8 +588,10 @@ Lemma BuildDFFun_is_syntax_ok
       (numRepArgs : nat)
       wrappedRep
       (progOK : {prog : Stmt &
-                        LiftMethod (Cod := cod) (Dom := dom) env RepInv (DecomposeRep wrappedRep)
-                                   WrappedCod WrappedDom prog meth
+                        (forall env_ext,
+                            LiftMethod (Cod := cod) (Dom := dom) (env env_ext)
+                                       RepInv (DecomposeRep wrappedRep)
+                                       WrappedCod WrappedDom prog meth)
                         (* Syntactic Checks *)
                         /\ NoUninitDec.is_no_uninited
                              {|
@@ -589,7 +643,9 @@ Qed.
 
 Definition BuildDFFun
            av
-           (env : Env av)
+           (* The calling environment is parameterized over an extension *)
+           (* representing the operational specifications of the module. *)
+           (env : StringMap.t DFFun -> Env av)
            {WrappedRepT RepT}
            cod
            dom
@@ -601,8 +657,9 @@ Definition BuildDFFun
            (numRepArgs : nat)
            wrappedRep
            (progOK : {prog : Stmt &
-                             LiftMethod (Cod := cod) (Dom := dom) env RepInv (DecomposeRep wrappedRep)
-                                        WrappedCod WrappedDom prog meth
+                             (forall env_ext,
+                             LiftMethod (Cod := cod) (Dom := dom) (env env_ext) RepInv (DecomposeRep wrappedRep)
+                                        WrappedCod WrappedDom prog meth)
                              (* Syntactic Checks *)
                              /\ NoUninitDec.is_no_uninited
                                   {|
@@ -636,12 +693,14 @@ Definition BuildDFFun
                 syntax_ok := proj2 (proj2 (proj2 (proj2 (proj2 (projT2 progOK)))))
 
              |};
-     compiled_syntax_ok := BuildDFFun_is_syntax_ok _ _ _ _
+     compiled_syntax_ok := BuildDFFun_is_syntax_ok _ _ _ _ progOK
   |}.
 
 Definition BuildFun
            av
-           (env : Env av)
+           (* The calling environment is parameterized over an extension *)
+           (* representing the operational specifications of the module. *)
+           (env : StringMap.t DFFun -> Env av)
            {WrappedRepT}
            {n n'}
            {consSigs : Vector.t consSig n}
@@ -655,8 +714,9 @@ Definition BuildFun
            wrappedRep
            (progsOK : forall midx,
                {prog : Stmt &
-                       LiftMethod env P (DecomposeRep wrappedRep)
-                                  (codWrap midx) (domWrap midx) prog (Methods adt midx)
+                       (forall env_ext,
+                       LiftMethod (env env_ext) P (DecomposeRep wrappedRep)
+                                  (codWrap midx) (domWrap midx) prog (Methods adt midx))
                        (* Syntactic Checks *)
                        /\ NoUninitDec.is_no_uninited
                             {|
@@ -681,7 +741,7 @@ Definition BuildFun
                        /\ is_syntax_ok prog = true} )
   : StringMap.t DFFun :=
   List.fold_left (fun acc el => StringMap.add (methID (Vector.nth methSigs el))
-                                              (BuildDFFun DecomposeRep
+                                              (BuildDFFun env DecomposeRep
                                                           _ wrappedRep (progsOK el) ) acc) (BuildFinUpTo n') (StringMap.empty _).
 
 Lemma AxiomatizeMethodPostSpec_OK
@@ -1029,7 +1089,7 @@ Arguments BuildArgNames !n !m / .
 
 Lemma compiled_prog_op_refines_ax
       av
-      (env : Env av)
+      (env : StringMap.t DFFun -> Env av)
       {numRepArgs}
       {A}
       {B}
@@ -1061,10 +1121,10 @@ Lemma compiled_prog_op_refines_ax
       (ValidMeth : refineMethod AbsR methSpec methImpl)
       RepInv
       progOK
-  :
+  : forall env_ext,
     op_refines_ax
-      env
-      (Core (BuildDFFun (env := env) (cod := cod) (dom := dom)
+      (env env_ext)
+      (Core (BuildDFFun env (cod := cod) (dom := dom)
                         (WrappedCod := codWrap) (WrappedDom := domWrap)
                         (meth := methImpl) (RepInv := RepInv)
                         DecomposeRep numRepArgs RepWrapper progOK))
@@ -1131,12 +1191,12 @@ Proof.
     remember DecomposeRep.
     assert (forall r,
                RepInv r ->
-               LiftMethod' env dom RepInv
+               LiftMethod' (env env_ext) dom RepInv
                            (fun r0 => list2Telescope (DecomposeRep RepWrapper r0))
                            (l0 RepWrapper r)
                            codWrap domWrap
                            prog l' (methImpl r)) as op_spec'
-        by (subst; exact op_spec); clear op_spec.
+        by (subst; exact (op_spec env_ext)); clear op_spec.
     clear Heql0.
     generalize l l' DecomposeRep DecomposeRepPre l0 op_spec' len_l_l' H''.
     clear methSpec ValidMeth l l' DecomposeRep DecomposeRepPre l0 op_spec' len_l_l' H''.
@@ -1252,12 +1312,12 @@ Proof.
     remember DecomposeRep.
     assert (forall r,
                RepInv r ->
-               LiftMethod' env dom RepInv
+               LiftMethod' (env env_ext) dom RepInv
                            (fun r0 => list2Telescope (DecomposeRep RepWrapper r0))
                            (l0 RepWrapper r)
                            codWrap domWrap
                            prog l' (methImpl r)) as op_spec'
-        by (subst; exact op_spec); clear op_spec.
+        by (subst; exact (op_spec env_ext)); clear op_spec.
     replace (@nil (prod (Value av) (option av))) with (map (fun v : Value av => (v, @None av)) l) by
         (subst; destruct l; simpl in *; congruence).
     clear Heql'; clear Heql0.
@@ -1987,6 +2047,7 @@ Proof.
     apply mem_in_iff; eauto.
 Qed.
 
+
 Lemma BuildCompileUnit2T_exports_in_domain
       av
       (env : GLabelMap.t (AxiomaticSpec av))
@@ -2016,16 +2077,21 @@ Lemma BuildCompileUnit2T_exports_in_domain
       (DecomposeRepPrePoseAgree := fun r r' =>
                                      DecomposePrei3list_Agree av RepT RepWrapper (RepMap r) (RepMap r'))
       (env'' :=
-         (GLabelMapFacts.UWFacts.WFacts.P.update
-            (GLabelMap.map (Axiomatic (ADTValue:=av))
-                           (map_aug_mod_name op_mod_name'
-                                             (GenExports codWrap domWrap AbsR RepInv DecomposeRepPre
-                                                         DecomposeRepPost DecomposeRepPrePoseAgree ValidImpl)))
-            env'))
+                fun env''' : StringMap.t DFFun =>
+                (GLabelMapFacts.UWFacts.WFacts.P.update
+                   (GLabelMapFacts.UWFacts.WFacts.P.update
+                      (GLabelMap.map (fun f : DFFun => Operational av f)
+                                     (map_aug_mod_name op_mod_name' env'''))
+                      (GLabelMap.map (Axiomatic (ADTValue:=av))
+                                  (map_aug_mod_name op_mod_name'
+                                                    (GenExports codWrap domWrap AbsR RepInv DecomposeRepPre
+                                                                DecomposeRepPost DecomposeRepPrePoseAgree ValidImpl))))
+                   env'))
       (progsOK : forall midx,
           {prog : Stmt &
-                  LiftMethod env'' RepInv (DecomposeRep RepWrapper)
-                             (codWrap midx) (domWrap midx) prog (Methods adtImpl midx)
+                  (forall env_ext,
+                      LiftMethod (env'' env_ext) RepInv (DecomposeRep RepWrapper)
+                                 (codWrap midx) (domWrap midx) prog (Methods adtImpl midx))
                   (* Syntactic Checks *)
                   /\ NoUninitDec.is_no_uninited
                        {|
@@ -2057,7 +2123,7 @@ Lemma BuildCompileUnit2T_exports_in_domain
   : is_sub_domain
       (GenExports codWrap domWrap AbsR RepInv DecomposeRepPre
                   DecomposeRepPost DecomposeRepPrePoseAgree ValidImpl)
-      (BuildFun adtImpl DecomposeRep numRepArgs codWrap domWrap
+      (BuildFun _ adtImpl DecomposeRep numRepArgs codWrap domWrap
                 RepWrapper progsOK).
 Proof.
   simpl.
@@ -2123,16 +2189,21 @@ Lemma BuildCompileUnit2T_projT2
       (DecomposeRepPrePoseAgree := fun r r' =>
                                      DecomposePrei3list_Agree av RepT RepWrapper (RepMap r) (RepMap r'))
       (env'' :=
-         (GLabelMapFacts.UWFacts.WFacts.P.update
-            (GLabelMap.map (Axiomatic (ADTValue:=av))
-                           (map_aug_mod_name op_mod_name'
-                                             (GenExports codWrap domWrap AbsR RepInv DecomposeRepPre
-                                                         DecomposeRepPost DecomposeRepPrePoseAgree ValidImpl)))
-            env'))
+         fun env''' : StringMap.t DFFun =>
+           (GLabelMapFacts.UWFacts.WFacts.P.update
+              (GLabelMapFacts.UWFacts.WFacts.P.update
+                 (GLabelMap.map (fun f : DFFun => Operational av f)
+                                (map_aug_mod_name op_mod_name' env'''))
+                 (GLabelMap.map (Axiomatic (ADTValue:=av))
+                                (map_aug_mod_name op_mod_name'
+                                                  (GenExports codWrap domWrap AbsR RepInv DecomposeRepPre
+                                                              DecomposeRepPost DecomposeRepPrePoseAgree ValidImpl))))
+              env'))
       (progsOK : forall midx,
           {prog : Stmt &
-                  LiftMethod env'' RepInv (DecomposeRep RepWrapper)
-                             (codWrap midx) (domWrap midx) prog (Methods adtImpl midx)
+                  (forall env_ext,
+                      LiftMethod (env'' env_ext) RepInv (DecomposeRep RepWrapper)
+                                 (codWrap midx) (domWrap midx) prog (Methods adtImpl midx))
                   (* Syntactic Checks *)
                   /\ NoUninitDec.is_no_uninited
                        {|
@@ -2172,12 +2243,13 @@ Lemma BuildCompileUnit2T_projT2
        : forallb NameDecoration.is_good_module_name
                  (map (fun x => fst (fst x)) (GLabelMap.elements  env)) = true)
       proof
-  : CompileUnit2Equiv env'' adtImpl RepInv DecomposeRep numRepArgs ax_mod_name'
+      env_ext
+  : CompileUnit2Equiv (env'' env_ext) adtImpl RepInv DecomposeRep numRepArgs ax_mod_name'
                       op_mod_name' codWrap domWrap RepWrapper
                       {|
                         module := {|
                                    Imports := env;
-                                   Funs := BuildFun adtImpl DecomposeRep numRepArgs codWrap domWrap
+                                   Funs := BuildFun _ adtImpl DecomposeRep numRepArgs codWrap domWrap
                                                     RepWrapper progsOK;
                                    import_module_names_good := no_cito_clash_env |};
                         ax_mod_name := ax_mod_name';
@@ -2194,170 +2266,183 @@ Lemma BuildCompileUnit2T_projT2
 Proof.
   unfold CompileUnit2Equiv; repeat split; simpl; eauto.
   unfold DFModuleEquiv; intros.
-  eexists (BuildDFFun DecomposeRep _ RepWrapper (progsOK midx)).
+  eexists (BuildDFFun _ DecomposeRep _ RepWrapper (progsOK midx)).
   simpl. repeat split.
   intros.
-  eapply (proj1 (projT2 (progsOK midx)) r H).
+  eapply (proj1 (projT2 (progsOK midx)) _ r H).
   unfold BuildFun.
   eapply (@StringMapsTo_fold_left' _ _ (fun el => methID (Vector.nth methSigs el))
-                                   (fun el => BuildDFFun DecomposeRep numRepArgs RepWrapper (progsOK el))).
+                                   (fun el => BuildDFFun _ DecomposeRep numRepArgs RepWrapper (progsOK el))).
   apply methID_injective; eauto.
 Qed.
 
-Lemma BuildCompileUnit2T_proof
-      av
-      (env : GLabelMap.t (AxiomaticSpec av))
-      (env' := GLabelMap.map (@Axiomatic av) env)
-      {n n'}
-      {consSigs : Vector.t consSig n}
-      {methSigs : Vector.t methSig n'}
-      (UniqueMeth : NoDup (Vector.to_list (Vector.map methID methSigs)))
-      (adtSpec adtImpl : DecoratedADT (BuildADTSig consSigs methSigs))
-      {numRepArgs}
-      {A}
-      {B}
-      {C}
-      {RepT' : Vector.t A numRepArgs}
-      (RepT : ilist3 (B := B) RepT')
-      (RepWrapper : @RepWrapperT av numRepArgs A B C RepT' RepT)
-      (RepMap : Rep adtImpl -> i3list C RepT)
-      (ValidImpl : refineADT adtSpec adtImpl)
-      (AbsR' := AbsR ValidImpl)
-      RepInv
-      (DecomposeRep := fun repWrapper rep => Decomposei3list RepT' RepT repWrapper (RepMap rep))
-      (DecomposeRepPre := fun rep => DecomposePrei3list RepT' RepT RepWrapper (RepMap rep))
-      (DecomposeRepPost := fun rep rep' => DecomposePosti3list _ RepT RepWrapper (RepMap rep) (RepMap rep'))
-      ax_mod_name'
-      op_mod_name'
-      codWrap
-      domWrap
-      (DecomposeRepPrePoseAgree := fun r r' =>
-                                     DecomposePrei3list_Agree av RepT RepWrapper (RepMap r) (RepMap r'))
-      (env'' :=
-         (GLabelMapFacts.UWFacts.WFacts.P.update
-            (GLabelMap.map (Axiomatic (ADTValue:=av))
-                           (map_aug_mod_name op_mod_name'
-                                             (GenExports codWrap domWrap AbsR' RepInv DecomposeRepPre
-                                                         DecomposeRepPost DecomposeRepPrePoseAgree ValidImpl)))
-            env'))
-      (progsOK : forall midx,
-          {prog : Stmt &
-                  LiftMethod env'' RepInv (DecomposeRep RepWrapper)
-                             (codWrap midx) (domWrap midx) prog (Methods adtImpl midx)
-                  (* Syntactic Checks *)
-                  /\ NoUninitDec.is_no_uninited
-                       {|
-                         FuncCore.ArgVars := BuildArgNames (Datatypes.length (fst
-                                                                                (MethodDomCod
-                                                                                   (BuildADTSig consSigs methSigs) midx)))
-                                                           numRepArgs;
-                         FuncCore.RetVar := "ret";
-                         FuncCore.Body := Compile.compile
-                                            (CompileDFacade.compile prog) |} = true
-                  /\ (GoodModuleDec.is_arg_len_ok
-                        (Compile.compile (CompileDFacade.compile prog)) = true)
-                  /\ (GoodModuleDec.is_good_size
-                        (Datatypes.length
-                           (GetLocalVars.get_local_vars
-                              (Compile.compile (CompileDFacade.compile prog))
-                              (BuildArgNames (Datatypes.length (fst
-                                                                  (MethodDomCod
-                                                                     (BuildADTSig consSigs methSigs) midx))) numRepArgs) "ret") +
-                         Depth.depth (Compile.compile (CompileDFacade.compile prog))) =
-                      true)
-                  /\  is_disjoint (assigned prog)
-                                  (StringSetFacts.of_list
+ Lemma BuildCompileUnit2T_proof
+                     av
+             (env : GLabelMap.t (AxiomaticSpec av))
+             (env' := GLabelMap.map (@Axiomatic av) env)
+             {n n'}
+             {consSigs : Vector.t consSig n}
+             {methSigs : Vector.t methSig n'}
+             (UniqueMeth : NoDup (Vector.to_list (Vector.map methID methSigs)))
+             (adtSpec adtImpl : DecoratedADT (BuildADTSig consSigs methSigs))
+             {numRepArgs}
+             {A}
+             {B}
+             {C}
+             {RepT' : Vector.t A numRepArgs}
+             (RepT : ilist3 (B := B) RepT')
+             (RepWrapper : @RepWrapperT av numRepArgs A B C RepT' RepT)
+             (RepMap : Rep adtImpl -> i3list C RepT)
+             (ValidImpl : refineADT adtSpec adtImpl)
+             (AbsR' := AbsR ValidImpl)
+             RepInv
+             (DecomposeRep :=
+                fun repWrapper rep =>
+                  Decomposei3list RepT' RepT repWrapper (RepMap rep))
+             (DecomposeRepPre :=
+                fun rep =>
+                  DecomposePrei3list RepT' RepT RepWrapper (RepMap rep))
+             (DecomposeRepPost :=
+                fun rep rep' =>
+                  DecomposePosti3list _ RepT RepWrapper (RepMap rep) (RepMap rep'))
+             ax_mod_name'
+             op_mod_name'
+             codWrap
+             domWrap
+             (DecomposeRepPrePoseAgree :=
+                fun r r' =>
+                  DecomposePrei3list_Agree av RepT RepWrapper (RepMap r) (RepMap r'))
+             (env'' :=
+                fun env''' =>
+                (GLabelMapFacts.UWFacts.WFacts.P.update
+                   (GLabelMapFacts.UWFacts.WFacts.P.update
+                      (GLabelMap.map (fun f : DFFun => Operational av f)
+                                     (map_aug_mod_name op_mod_name' env'''))
+                      (GLabelMap.map (Axiomatic (ADTValue:=av))
+                                  (map_aug_mod_name op_mod_name'
+                                                    (GenExports codWrap domWrap AbsR' RepInv DecomposeRepPre
+                                                                DecomposeRepPost DecomposeRepPrePoseAgree ValidImpl))))
+                   env'))
+
+             (progsOK : forall midx,
+                 {prog : Stmt &
+                         (forall env_ext,
+                         LiftMethod (env'' env_ext) RepInv (DecomposeRep RepWrapper)
+                                    (codWrap midx) (domWrap midx) prog (Methods adtImpl midx))
+                         (* Syntactic Checks *)
+                         /\ NoUninitDec.is_no_uninited
+                              {|
+                                FuncCore.ArgVars := BuildArgNames (Datatypes.length (fst
+                                                                                       (MethodDomCod
+                                                                                          (BuildADTSig consSigs methSigs) midx)))
+                                                                  numRepArgs;
+                                FuncCore.RetVar := "ret";
+                                FuncCore.Body := Compile.compile
+                                                   (CompileDFacade.compile prog) |} = true
+                         /\ (GoodModuleDec.is_arg_len_ok
+                               (Compile.compile (CompileDFacade.compile prog)) = true)
+                         /\ (GoodModuleDec.is_good_size
+                               (Datatypes.length
+                                  (GetLocalVars.get_local_vars
+                                     (Compile.compile (CompileDFacade.compile prog))
                                      (BuildArgNames (Datatypes.length (fst
                                                                          (MethodDomCod
-                                                                            (BuildADTSig consSigs methSigs) midx)))
-                                                    numRepArgs)) = true
-                  /\ is_syntax_ok prog = true} )
-      (distinct_mod_name : negb (ListFacts3.string_bool ax_mod_name' op_mod_name') = true)
-      (unique_op_mod_name'
-       : forallb (fun x : string => negb (ListFacts3.string_bool op_mod_name' x))
-                 (map (fun x : string * string * AxiomaticSpec av => fst (fst x))
-                      (GLabelMap.elements (elt:=AxiomaticSpec av) env)) = true)
-      (no_cito_clash_op_mod
-       : negb (prefix "__cmod_impl_" op_mod_name') = true)
-      (no_cito_clash_env
-       : forallb NameDecoration.is_good_module_name
-                 (map (fun x => fst (fst x)) (GLabelMap.elements  env)) = true)
-  : ops_refines_axs
-      (get_env op_mod_name'
-               (GenExports
-                  codWrap domWrap AbsR' RepInv
-                  (fun rep : Rep adtImpl =>
-                     DecomposePrei3list RepT' RepT RepWrapper (RepMap rep))
-                  (fun rep rep' : Rep adtImpl =>
-                     DecomposePosti3list RepT' RepT RepWrapper
-                                         (RepMap rep) (RepMap rep'))
-                  (fun r r' : Rep adtImpl =>
-                     DecomposePrei3list_Agree av RepT RepWrapper
-                                              (RepMap r) (RepMap r'))
-                  ValidImpl)
-               {|
-                 Imports := env;
-                 Funs := BuildFun adtImpl DecomposeRep numRepArgs codWrap domWrap
-                                  RepWrapper progsOK;
-                 import_module_names_good := no_cito_clash_env |})
-      (StringMap.map Core
-                     (Funs
-                        {|
-                          Imports := env;
-                          Funs := BuildFun adtImpl DecomposeRep numRepArgs codWrap domWrap
-                                           RepWrapper progsOK;
-                          import_module_names_good := no_cito_clash_env |}))
-      (GenExports codWrap
-                  domWrap AbsR' RepInv
-                  (fun rep : Rep adtImpl =>
-                     DecomposePrei3list RepT' RepT RepWrapper (RepMap rep))
-                  (fun rep rep' : Rep adtImpl =>
-                     DecomposePosti3list RepT' RepT RepWrapper (RepMap rep) (RepMap rep'))
-                  (fun r r' : Rep adtImpl =>
-                     DecomposePrei3list_Agree av RepT RepWrapper (RepMap r) (RepMap r'))
-                  ValidImpl).
-Proof.
-  unfold ops_refines_axs; intros.
-  unfold GenExports in H.
-  assert (exists midx, x = methID (Vector.nth methSigs midx)).
-  setoid_rewrite <- find_mapsto_iff in H.
-  apply StringMapsTo_fold_left_ex in H; destruct_ex; intuition eauto.
-  eauto using methID_injective; eauto.
-  eapply ListFacts1.Injection_NoDup; eauto using NoDup_BuildFinUpTo.
-  eauto using methID_injective; eauto.
-  destruct H0; subst.
-  pose proof (@StringMapsTo_fold_left'
-                _ _
-                (fun el => methID (Vector.nth methSigs el))
-                (fun el => GenAxiomaticSpecs AbsR' RepInv (codWrap el)
-                                             (domWrap el) (Methods adtSpec el) DecomposeRepPre DecomposeRepPost
-                                             DecomposeRepPrePoseAgree) ∅ x0 (methID_injective _ UniqueMeth)).
-  setoid_rewrite find_mapsto_iff in H0.
-  subst DecomposeRepPre; subst DecomposeRepPost; subst DecomposeRepPrePoseAgree.
-  assert (Some ax_spec = Some
-                           (GenAxiomaticSpecs AbsR' RepInv (codWrap x0)
-                                              (domWrap x0) (Methods adtSpec x0)
-                                              (fun rep =>
-                                                 DecomposePrei3list RepT' RepT RepWrapper (RepMap rep))
-                                              (fun rep rep' =>
-                                                 DecomposePosti3list RepT' RepT RepWrapper
-                                                                     (RepMap rep) (RepMap rep'))
-                                              (fun r r' =>
-                                                 DecomposePrei3list_Agree av RepT RepWrapper
-                                                                          (RepMap r) (RepMap r')))) by
-      (rewrite <- H, <- H0; f_equal).
-  injections.
-  eexists; intuition.
-  unfold Funs.
-  unfold BuildFun.
-  setoid_rewrite <- find_mapsto_iff.
-  eapply StringMap.map_1.
-  eapply (@StringMapsTo_fold_left' _ _ (fun el => methID (Vector.nth methSigs el))
-                                   (fun el => BuildDFFun DecomposeRep numRepArgs RepWrapper (progsOK el))).
-  apply methID_injective; eauto.
-  apply compiled_prog_op_refines_ax.
-  apply (ADTRefinementPreservesMethods ValidImpl x0).
-Qed.
+                                                                            (BuildADTSig consSigs methSigs) midx))) numRepArgs) "ret") +
+                                Depth.depth (Compile.compile (CompileDFacade.compile prog))) =
+                             true)
+                         /\  is_disjoint (assigned prog)
+                                         (StringSetFacts.of_list
+                                            (BuildArgNames (Datatypes.length (fst
+                                                                                (MethodDomCod
+                                                                                   (BuildADTSig consSigs methSigs) midx)))
+                                                           numRepArgs)) = true
+                         /\ is_syntax_ok prog = true} )
+             (distinct_mod_name : negb (ListFacts3.string_bool ax_mod_name' op_mod_name') = true)
+             (unique_op_mod_name'
+              : forallb (fun x : string => negb (ListFacts3.string_bool op_mod_name' x))
+                        (map (fun x : string * string * AxiomaticSpec av => fst (fst x))
+                             (GLabelMap.elements (elt:=AxiomaticSpec av) env)) = true)
+             (no_cito_clash_op_mod
+              : negb (prefix "__cmod_impl_" op_mod_name') = true)
+             (no_cito_clash_env
+              : forallb NameDecoration.is_good_module_name
+                        (map (fun x => fst (fst x)) (GLabelMap.elements  env)) = true)
+    : ops_refines_axs
+     (get_env op_mod_name'
+        (GenExports
+           codWrap domWrap AbsR' RepInv
+           (fun rep : Rep adtImpl =>
+            DecomposePrei3list RepT' RepT RepWrapper (RepMap rep))
+           (fun rep rep' : Rep adtImpl =>
+            DecomposePosti3list RepT' RepT RepWrapper
+              (RepMap rep) (RepMap rep'))
+           (fun r r' : Rep adtImpl =>
+            DecomposePrei3list_Agree av RepT RepWrapper
+                                     (RepMap r) (RepMap r'))
+           ValidImpl)
+        {|
+        Imports := env;
+        Funs := BuildFun _ adtImpl DecomposeRep numRepArgs codWrap domWrap
+                  RepWrapper progsOK;
+        import_module_names_good := no_cito_clash_env |})
+     (StringMap.map Core
+        (Funs
+           {|
+           Imports := env;
+           Funs := BuildFun _ adtImpl DecomposeRep numRepArgs codWrap domWrap
+                     RepWrapper progsOK;
+           import_module_names_good := no_cito_clash_env |}))
+     (GenExports codWrap
+        domWrap AbsR' RepInv
+        (fun rep : Rep adtImpl =>
+         DecomposePrei3list RepT' RepT RepWrapper (RepMap rep))
+        (fun rep rep' : Rep adtImpl =>
+         DecomposePosti3list RepT' RepT RepWrapper (RepMap rep) (RepMap rep'))
+        (fun r r' : Rep adtImpl =>
+           DecomposePrei3list_Agree av RepT RepWrapper (RepMap r) (RepMap r'))
+        ValidImpl).
+  Proof.
+    unfold ops_refines_axs; intros.
+    unfold GenExports in H.
+    assert (exists midx, x = methID (Vector.nth methSigs midx)).
+    setoid_rewrite <- find_mapsto_iff in H.
+    apply StringMapsTo_fold_left_ex in H; destruct_ex; intuition eauto.
+    eauto using methID_injective; eauto.
+    eapply ListFacts1.Injection_NoDup; eauto using NoDup_BuildFinUpTo.
+    eauto using methID_injective; eauto.
+    destruct H0; subst.
+    pose proof (@StringMapsTo_fold_left'
+            _ _
+            (fun el => methID (Vector.nth methSigs el))
+            (fun el => GenAxiomaticSpecs AbsR' RepInv (codWrap el)
+              (domWrap el) (Methods adtSpec el) DecomposeRepPre DecomposeRepPost
+              DecomposeRepPrePoseAgree) ∅ x0 (methID_injective _ UniqueMeth)).
+    setoid_rewrite find_mapsto_iff in H0.
+    subst DecomposeRepPre; subst DecomposeRepPost; subst DecomposeRepPrePoseAgree.
+    assert (Some ax_spec = Some
+         (GenAxiomaticSpecs AbsR' RepInv (codWrap x0)
+            (domWrap x0) (Methods adtSpec x0)
+            (fun rep =>
+             DecomposePrei3list RepT' RepT RepWrapper (RepMap rep))
+            (fun rep rep' =>
+             DecomposePosti3list RepT' RepT RepWrapper
+               (RepMap rep) (RepMap rep'))
+            (fun r r' =>
+             DecomposePrei3list_Agree av RepT RepWrapper
+               (RepMap r) (RepMap r')))) by
+        (rewrite <- H, <- H0; f_equal).
+    injections.
+    eexists; intuition.
+    unfold Funs.
+    unfold BuildFun.
+    setoid_rewrite <- find_mapsto_iff.
+    eapply StringMap.map_1.
+    eapply (@StringMapsTo_fold_left' _ _ (fun el => methID (Vector.nth methSigs el))
+         (fun el => BuildDFFun _ DecomposeRep numRepArgs RepWrapper (progsOK el))).
+    apply methID_injective; eauto.
+    apply compiled_prog_op_refines_ax with (env := env'').
+    apply (ADTRefinementPreservesMethods ValidImpl x0).
+  Qed.
 
 (* This is the main compilation tool. *)
 Definition BuildCompileUnit2T'
@@ -2391,16 +2476,21 @@ Definition BuildCompileUnit2T'
            (DecomposeRepPrePoseAgree := fun r r' =>
                                           DecomposePrei3list_Agree av RepT RepWrapper (RepMap r) (RepMap r'))
            (env'' :=
-              (GLabelMapFacts.UWFacts.WFacts.P.update
-                 (GLabelMap.map (Axiomatic (ADTValue:=av))
-                                (map_aug_mod_name op_mod_name'
-                                                  (GenExports codWrap domWrap AbsR' RepInv DecomposeRepPre
-                                                              DecomposeRepPost DecomposeRepPrePoseAgree ValidImpl)))
-                 env'))
+                fun env''' =>
+                (GLabelMapFacts.UWFacts.WFacts.P.update
+                   (GLabelMapFacts.UWFacts.WFacts.P.update
+                      (GLabelMap.map (fun f : DFFun => Operational av f)
+                                     (map_aug_mod_name op_mod_name' env'''))
+                      (GLabelMap.map (Axiomatic (ADTValue:=av))
+                                  (map_aug_mod_name op_mod_name'
+                                                    (GenExports codWrap domWrap AbsR' RepInv DecomposeRepPre
+                                                                DecomposeRepPost DecomposeRepPrePoseAgree ValidImpl))))
+                   env'))
            (progsOK : forall midx,
                {prog : Stmt &
-                       LiftMethod env'' RepInv (DecomposeRep RepWrapper)
-                                  (codWrap midx) (domWrap midx) prog (Methods adtImpl midx)
+                       (forall env_ext,
+                           LiftMethod (env'' env_ext) RepInv (DecomposeRep RepWrapper)
+                                      (codWrap midx) (domWrap midx) prog (Methods adtImpl midx))
                        (* Syntactic Checks *)
                        /\ NoUninitDec.is_no_uninited
                             {|
@@ -2439,7 +2529,8 @@ Definition BuildCompileUnit2T'
            (no_cito_clash_env
             : forallb NameDecoration.is_good_module_name
                       (map (fun x => fst (fst x)) (GLabelMap.elements  env)) = true)
-  : BuildCompileUnit2TSpec env''
+
+  : BuildCompileUnit2TSpec (env'' (StringMap.empty _))
                            AbsR'
                            RepInv
                            DecomposeRep
@@ -2455,7 +2546,7 @@ Definition BuildCompileUnit2T'
                            ValidImpl.
 Proof.
   eexists {| module := {| Funs :=
-                            BuildFun
+                            BuildFun _
                               adtImpl DecomposeRep _ codWrap domWrap
                               RepWrapper progsOK;
                           Imports := _;
